pulse/lib/steel/pulse/Pulse.Checker.Bind.fsti
@@ -20,9 +20,9 @@ val mk_bind (g:env)
             (px:nvar { ~ (snd px `Set.mem` dom g) })
             (d_e1:st_typing g e1 c1)
             (d_c1res:tot_typing g (comp_res c1) (tm_type (comp_u c1)))
-            (d_e2:st_typing (push_binding g (snd px) (comp_res c1)) (open_st_term_nv e2 px) c2)
+            (d_e2:st_typing (push_binding g (snd px) (fst px) (comp_res c1)) (open_st_term_nv e2 px) c2)
             (res_typing:universe_of g (comp_res c2) (comp_u c2))
-            (post_typing:tot_typing (push_binding g (snd px) (comp_res c2)) (open_term_nv (comp_post c2) px) Tm_VProp)
+            (post_typing:tot_typing (push_binding g (snd px) (fst px) (comp_res c2)) (open_term_nv (comp_post c2) px) Tm_VProp)
   : T.TacH (t:st_term &
             c:comp_st { st_comp_of_comp c == st_comp_with_pre (st_comp_of_comp c2) pre } &
             st_typing g t c)
@@ -39,7 +39,7 @@ val bind_res_and_post_typing (g:env) (s2:st_comp)
                              (x:var { Pulse.Typing.Metatheory.fresh_wrt x g (freevars s2.post) })
                              (post_hint:post_hint_opt g { comp_post_matches_hint (C_ST s2) post_hint })
   : T.Tac (universe_of g s2.res s2.u &
-           tot_typing (push_binding g x s2.res) (open_term_nv s2.post (v_as_nv x)) Tm_VProp)
+           tot_typing (push_binding g x ppname_default s2.res) (open_term_nv s2.post (v_as_nv x)) Tm_VProp)
 
 val check_bind (g:env)
                (t:st_term{Tm_Bind? t.term})
