pulse/share/steel/examples/pulse/bug-reports/ExistsWitness.fst
@@ -25,7 +25,7 @@ let assume_squash (p:prop) : squash p = assume p
 //it adds an extra level of reveal/hide around it
 //and this causes the match to fail; although one would expect
 //F* to cancel the additional layer of reveal/hide
-[@@expect_failure]    
+//[@@expect_failure]    
 ```pulse
 fn sample (x:R.ref int)
 requires exists p y. R.pts_to x p y
@@ -38,7 +38,7 @@ ensures exists p y. R.pts_to x p y ** pure (y == 17)
 ```
 
 ```pulse
-fn sample (x:R.ref int) (#p:perm)
+fn sample_ (x:R.ref int) (#p:perm)
 requires exists y. R.pts_to x p y
 ensures exists y. R.pts_to x p y ** pure (y == 17)
 {
